examples/map/MapIAproof.v
@@ -33,6 +33,7 @@ End MapIA. End MapIA.
 Module w_MapIA. Section w_MapIA.
   Context `{!invG α Σ Γ, !subG Γ Σ, !sinvG Σ Γ α β τ, !MapAGΓ Γ, !MapMGΓ Γ, !memGΓ Γ}.
   Context (n : level).
+
   Theorem correct gi (SpcMap : univ_id → string → option fspec) (SpcMem : string → option fspec)
       (MapInSpcMap : ∀ υ, spc_incl (MapAS.Spc υ n) (SpcMap υ)) :
     w_ctx_refines
@@ -44,20 +45,11 @@ Module w_MapIA. Section w_MapIA.
       instantiate (1:= λ u, to_spc (MapMS.Spc u%positive n)).
       i. split; try refl. unfold MapMS.Spc. unseal CRIS. prove_nodup.
     }
-    etrans; cycle 1.
-    { eapply w_ctx_refines_frameR.
-      rewrite -(hmod_addc_empty_l _ MapM.InitCond).
-      etrans; first eapply wctxr.
-      {  }
-      rewrite -[MapM.InitCond]/(MapM.InitCond ∗ emp)%I.
-      instantiate (1:=(emp%I ∗ MapM.InitCond)%I).
-      eapply w_ctx_refines_cond_frameR.
-      (* rewrite -(hmod_addc_empty_l _ MapM.InitCond). *)
-      eapply ctxr_cond_frameR, main_adequacy, MapMA.sim; eauto.
-      split; try refl.
-      rewrite /MapMS.Spc; unseal CRIS; prove_nodup.
-    }
-    refl.
-  Unshelve. r; lia.
+    eapply w_ctx_refines_frameR.
+    eapply w_ctx_refines_cond_strengthen; first (instantiate (1:=(emp ∗ MapM.InitCond)%I)).
+    { iIntros "[_ $]". }
+    eapply w_ctx_refines_cond_frameR, wctxr; eauto.
+    split; try refl.
+    rewrite /MapMS.Spc; unseal CRIS; prove_nodup.
   Qed.
 End w_MapIA. End w_MapIA.
